\begin{proof} \hfill\par
    \begin{tabular}{rll}
        1. & \( p \lor r \to (q \to s) \) & [ Given ] \\
        2. & \( p \lor r \to (\neg s \to \neg q) \) & [ Contrapositive: 1 ] \\
        3. & \( t \) & [ Given ] \\
        \multicolumn{3}{l}{\quad \begin{tabular}{rll}
            4.1. & \( r \) & [ Assumption ] \\
            4.2. & \( p \lor r \) & [ Intro \(\lor\): 4.1 ] \\
            4.3. & \( \neg s \to \neg q \) & [ Modus Ponens: 2, 4.2 ] \\
            4.4. & \( r \land t \) & [ Intro \(\land\): 3, 4.1 ] \\
            4.5. & \( r \land t \to \neg s \) & [ Given ] \\
            4.6. & \( \neg s \) & [ Modus Ponens: 4.4, 4.5 ] \\
            4.7. & \( \neg q \) & [ Modus Ponens: 4.3, 4.6 ] \\
        \end{tabular} } \\
        4. & \( r \to \neg q \) & [ Direct Proof Rule ] \\
    \end{tabular} \par
\end{proof}
